Test/dafny1/Induction.dfy
@@ -1,0 +1,132 @@
+class IntegerInduction {
+  // This class considers different ways of proving, for any natural n:
+  //   (SUM i in [0, n] :: i^3) == (SUM i in [0, n] :: i)^2
+
+  // In terms of Dafny functions, the theorem to be proved is:
+  //   SumOfCubes(n) == Gauss(n) * Gauss(n)
+
+  function SumOfCubes(n: int): int
+    requires 0 <= n;
+  {
+    if n == 0 then 0 else SumOfCubes(n-1) + n*n*n
+  }
+
+  function Gauss(n: int): int
+    requires 0 <= n;
+  {
+    if n == 0 then 0 else Gauss(n-1) + n
+  }
+
+  // Here is one proof.  It uses a lemma, which is proved separately.
+
+  ghost method Theorem0(n: int)
+    requires 0 <= n;
+    ensures SumOfCubes(n) == Gauss(n) * Gauss(n);
+  {
+    if (n != 0) {
+      call Theorem0(n-1);
+      call Lemma(n-1);
+    }
+  }
+
+  ghost method Lemma(n: int)
+    requires 0 <= n;
+    ensures 2 * Gauss(n) == n*(n+1);
+  {
+    if (n != 0) { call Lemma(n-1); }
+  }
+
+  // Here is another proof.  It states the lemma as part of the theorem, and
+  // thus proves the two together.
+
+  ghost method Theorem1(n: int)
+    requires 0 <= n;
+    ensures SumOfCubes(n) == Gauss(n) * Gauss(n);
+    ensures 2 * Gauss(n) == n*(n+1);
+  {
+    if (n != 0) {
+      call Theorem1(n-1);
+    }
+  }
+
+  // Here is another proof.  It makes use of Dafny's {:induction} attribute to
+  // prove the lemma.
+
+  ghost method Theorem2(n: int)
+    requires 0 <= n;
+    ensures SumOfCubes(n) == Gauss(n) * Gauss(n);
+  {
+    if (n != 0) {
+      call Theorem0(n-1);
+
+      assert (forall m {:induction} :: 0 <= m ==> 2 * Gauss(m) == m*(m+1));
+    }
+  }
+
+  ghost method M(n: int)
+    requires 0 <= n;
+  {
+    assume (forall k :: 0 <= k && k < n ==> 2 * Gauss(k) == k*(k+1));  // manually assume the induction hypothesis
+    assert 2 * Gauss(n) == n*(n+1);
+  }
+
+  // Another way to prove the lemma is to supply a postcondition on the Gauss function
+
+  ghost method Theorem3(n: int)
+    requires 0 <= n;
+    ensures SumOfCubes(n) == GaussWithPost(n) * GaussWithPost(n);
+  {
+    if (n != 0) {
+      call Theorem3(n-1);
+    }
+  }
+
+  function GaussWithPost(n: int): int
+    requires 0 <= n;
+    ensures 2 * GaussWithPost(n) == n*(n+1);
+  {
+    if n == 0 then 0 else GaussWithPost(n-1) + n
+  }
+
+  // Finally, with the postcondition of GaussWithPost, one can prove the entire theorem by induction
+
+  ghost method Theorem4()
+    ensures (forall n {:induction} :: 0 <= n ==> SumOfCubes(n) == GaussWithPost(n) * GaussWithPost(n));
+  {
+    // look ma, no hints!
+  }
+
+  ghost method Theorem5(n: int)
+    requires 0 <= n;
+    ensures SumOfCubes(n) == GaussWithPost(n) * GaussWithPost(n);
+  {
+    // the postcondition is a simple consequence of these quantified versions of the theorem:
+    if (*) {
+      assert (forall m {:induction} :: 0 <= m ==> SumOfCubes(m) == GaussWithPost(m) * GaussWithPost(m));
+    } else {
+      call Theorem4();
+    }
+  }
+}
+
+datatype Tree<T> {
+  Leaf(T);
+  Branch(Tree<T>, Tree<T>);
+}
+
+class DatatypeInduction<T> {
+  function LeafCount<T>(tree: Tree<T>): int
+  {
+    match tree
+    case Leaf(t) => 1
+    case Branch(left, right) => LeafCount(left) + LeafCount(right)
+  }
+
+  method Theorem0(tree: Tree<T>)
+    ensures 1 <= LeafCount(tree);
+  {
+    assert (forall t: Tree<T> {:induction} :: 1 <= LeafCount(t));
+  }
+
+  // see also Test/dafny0/DTypes.dfy for more variations of this example
+}
